theories/models/utp_cml_new/utp_cml_sorts.thy
@@ -36,42 +36,77 @@ instance by (intro_classes, auto simp add:VALUE_cmlm_def UTYPE_cmlm_def)
 
 end
 
+lift_definition MkCmlVal :: "cmlv \<Rightarrow> cmlm uval" is MkCmlv
+  by (metis VALUE_cmlm_def rangeI)
+
+lift_definition DestCmlVal :: "cmlm uval \<Rightarrow> cmlv" is DestCmlv .
+
+lemma MkCmlVal_inv [simp]: "DestCmlVal (MkCmlVal x) = x"
+  by (transfer, simp)
+
+lemma MkCmlVal_bset_inv [simp]: "DestCmlVal `\<^sub>b MkCmlVal `\<^sub>b A = A"
+  by (metis (no_types, hide_lams) MkCmlVal_inv bset.map_comp bset.map_cong0 bset.map_id0 comp_def id_apply)
+
+lemma DestCmlVal_inject: "DestCmlVal A = DestCmlVal B \<Longrightarrow> A = B"
+  by (transfer, auto simp add:VALUE_cmlm_def)
+  
+lift_definition MkCmlTyp :: "cmlt \<Rightarrow> cmlm utype" is MkCmlt
+  by (metis UTYPE_cmlm_def rangeI)
+
+lift_definition DestCmlTyp :: "cmlm utype \<Rightarrow> cmlt" is DestCmlt .
+
+lemma DestCmlType_dest [dest!]: 
+  "DestCmlTyp t = a \<Longrightarrow> t = MkCmlTyp a"
+  by (transfer, auto simp add:UTYPE_cmlm_def)
+
+lemma MkCmlTyp_inv [simp]: "DestCmlTyp (MkCmlTyp x) = x"
+  by (transfer, simp)
+
 instantiation cmlm :: DEFINED_MODEL
 begin
 
-lift_definition value_defined_cmlm :: "cmlm uval \<Rightarrow> bool" is
-"\<lambda> v. \<D> (DestCmlv v) \<and> (\<exists>t. DestCmlv v :\<^sub>v t)" .
+definition value_defined_cmlm :: "cmlm uval \<Rightarrow> bool" where
+"\<D>\<^sub>v(v) \<longleftrightarrow> \<D> (DestCmlVal v) \<and> (\<exists>t. DestCmlVal v :\<^sub>v DestCmlTyp t)"
 
 instance
-  by (intro_classes, transfer, auto simp add:VALUE_cmlm_def, metis cmlt_total)
-
+  apply (intro_classes, simp add: value_defined_cmlm_def)
+  apply (transfer, auto simp add:VALUE_cmlm_def, metis cmlt_total)
+done
 end
 
 instantiation cmlm :: TYPED_MODEL
 begin
 
-lift_definition type_rel_cmlm :: "cmlm uval \<Rightarrow> cmlm utype \<Rightarrow> bool"
-is "\<lambda> x t. DestCmlv x :\<^sub>v DestCmlt t" .
+definition type_rel_cmlm :: "cmlm uval \<Rightarrow> cmlm utype \<Rightarrow> bool" where
+"x : t \<longleftrightarrow> DestCmlVal x :\<^sub>v DestCmlTyp t"
 
 instance
-  apply (intro_classes)
-  apply (transfer)
-  apply (auto simp add:UTYPE_cmlm_def VALUE_cmlm_def)
-  apply (metis cmlt_total)
-  apply (transfer, auto simp add:VALUE_cmlm_def UTYPE_cmlm_def)
+  apply (intro_classes, simp add: type_rel_cmlm_def)
+  apply (metis DestCmlVal.rep_eq DestCmlv.simps Rep_uval_cases VALUE_cmlm_def cmlt_total rangeI value_defined_cmlm_def)
+  apply (simp add: type_rel_cmlm_def value_defined_cmlm_def)
 done
 end
 
+lemma value_defined_cmlm_alt_def:
+  "\<D>\<^sub>v v  \<longleftrightarrow> \<D> (DestCmlVal v) \<and> (\<exists>t. v : t)"
+  by (simp add: value_defined_cmlm_def type_rel_cmlm_def)
+
+lemma value_defined_cmlm_dest:
+  "\<D>\<^sub>v v \<Longrightarrow> \<D> (DestCmlVal v)"
+  by (simp add:value_defined_cmlm_alt_def)
+  
 instantiation cmlm :: BOT_SORT
 begin
 
 term "BotD \<circ> DestCmlt"
 
-lift_definition ubot_cmlm :: "cmlm utype \<Rightarrow> cmlm uval" is
-"MkCmlv \<circ> BotD \<circ> DestCmlt" by (simp add:VALUE_cmlm_def)
+definition ubot_cmlm :: "cmlm utype \<Rightarrow> cmlm uval" where
+"ubot_cmlm = MkCmlVal \<circ> BotD \<circ> DestCmlTyp"
 
 instance
-  by (intro_classes, (transfer, auto)+)
+  apply (intro_classes)
+  apply (auto simp add: ubot_cmlm_def value_defined_cmlm_def type_rel_cmlm_def)
+done
 
 end
 
@@ -80,18 +115,22 @@ subsection {* Bool sort instantiation *}
 instantiation cmlm :: BOOL_SORT
 begin
 
-lift_definition MkBool_cmlm :: "bool \<Rightarrow> cmlm uval" 
-is "\<lambda> x. MkCmlv (BoolD x)" by (simp add:VALUE_cmlm_def)
+definition MkBool_cmlm :: "bool \<Rightarrow> cmlm uval" where 
+"MkBool x = MkCmlVal (BoolD x)"
 
-lift_definition DestBool_cmlm :: "cmlm uval \<Rightarrow> bool" is
-"\<lambda> x. the (ProjBoolD (DestCmlv x))" .
+definition DestBool_cmlm :: "cmlm uval \<Rightarrow> bool" where
+"DestBool x = the (ProjBoolD (DestCmlVal x))"
 
-lift_definition BoolType_cmlm :: "cmlm utype" 
-is "MkCmlt BoolT" by (simp add:UTYPE_cmlm_def) 
+definition BoolType_cmlm :: "cmlm utype" where 
+"BoolType = MkCmlTyp BoolT" 
 
 instance 
   apply (intro_classes, unfold_locales)
-  apply (transfer, auto elim!:BoolD_type_cases simp add:VALUE_cmlm_def)+
+  apply (auto elim!:BoolD_type_cases simp add: MkBool_cmlm_def DestBool_cmlm_def 
+                    value_defined_cmlm_def type_rel_cmlm_def BoolType_cmlm_def)
+  apply (metis BoolD_type MkCmlTyp_inv)
+  apply (transfer)
+  apply (auto elim!:BoolD_type_cases simp add:VALUE_cmlm_def)+
 done
 
 end
@@ -99,25 +138,24 @@ end
 instantiation cmlm :: STR_SORT
 begin
 
-lift_definition MkStr_cmlm :: "string \<Rightarrow> cmlm uval" 
-is "MkCmlv \<circ> StringD" by (simp add:VALUE_cmlm_def)
+definition MkStr_cmlm :: "string \<Rightarrow> cmlm uval" where
+"MkStr = MkCmlVal \<circ> StringD"
 
-lift_definition DestStr_cmlm :: "cmlm uval \<Rightarrow> string" is 
-"ProjStringD \<circ> DestCmlv" .
+definition DestStr_cmlm :: "cmlm uval \<Rightarrow> string" where 
+"DestStr = ProjStringD \<circ> DestCmlVal"
 
-lift_definition StrType_cmlm :: "cmlm utype" 
-is "MkCmlt StringT" by (simp add:UTYPE_cmlm_def) 
+definition StrType_cmlm :: "cmlm utype" where 
+"StrType = MkCmlTyp StringT" 
 
 instance
   apply (intro_classes, unfold_locales)
-  apply (transfer,auto)
-  apply (metis (full_types) CharD_type ListD_type ex_map_conv)
-  apply (transfer,auto)
-  apply (transfer,auto,subst map_idI, simp)
+  apply (transfer, auto)
+  apply (auto simp add: value_defined_cmlm_def MkStr_cmlm_def StrType_cmlm_def DestStr_cmlm_def type_rel_cmlm_def)
+  apply (metis (erased, lifting) CharD_type ListD_type MkCmlTyp_inv ex_map_conv)
+  apply (subst map_idI, simp_all)
+  apply (subst map_idI)
   apply (auto)
-  apply (transfer, simp add:VALUE_cmlm_def, clarify, simp)
-  apply (erule ListT_type_cases, auto, subst map_idI)
-  apply (auto)
+  apply (transfer, simp add:VALUE_cmlm_def, clarify, auto)
 done
 end
 
@@ -126,17 +164,18 @@ subsection {* List sort instantiation *}
 instantiation cmlm :: LIST_SORT
 begin
 
-lift_definition MkList_cmlm :: "cmlm utype \<Rightarrow> cmlm uval list \<Rightarrow> cmlm uval" is
-"\<lambda> a xs. MkCmlv (ListD (DestCmlt a) (map DestCmlv xs))" by (simp add:UTYPE_cmlm_def VALUE_cmlm_def)
+definition MkList_cmlm :: "cmlm utype \<Rightarrow> cmlm uval list \<Rightarrow> cmlm uval" where
+"MkList a xs = MkCmlVal (ListD (DestCmlTyp a) (map DestCmlVal xs))"
 
-lift_definition DestList_cmlm :: "cmlm uval \<Rightarrow> cmlm uval list" is
-"\<lambda> x. map MkCmlv (the (ProjListD (DestCmlv x)))" by (auto simp add:VALUE_cmlm_def pred_list_def)
+definition DestList_cmlm :: "cmlm uval \<Rightarrow> cmlm uval list" where
+"DestList x = map MkCmlVal (the (ProjListD (DestCmlVal x)))"
 
-lift_definition ListType_cmlm :: "cmlm utype \<Rightarrow> cmlm utype" is
-"\<lambda> a. MkCmlt (ListT (DestCmlt a))" by (simp add:UTYPE_cmlm_def)
+definition ListType_cmlm :: "cmlm utype \<Rightarrow> cmlm utype" where
+"ListType a = MkCmlTyp (ListT (DestCmlTyp a))"
 
 instance
   apply (intro_classes, unfold_locales)
+  apply (simp_all add:value_defined_cmlm_def MkList_cmlm_def DestList_cmlm_def ListType_cmlm_def type_rel_cmlm_def WT_LIST_def)
   apply (auto simp add:WT_LIST_def)[1]
   apply (transfer, (auto simp add:UTYPE_cmlm_def)[1])
   apply (transfer, auto elim!:ListD_type_cases simp add:UTYPE_cmlm_def VALUE_cmlm_def)
@@ -148,30 +187,153 @@ instance
   apply (subst map_idI, auto, metis DestCmlv.simps list_all_iff rangeE)
   apply (transfer, auto simp add: VALUE_cmlm_def UTYPE_cmlm_def)
   apply (subst map_idI, auto)
-  apply (simp add: WT_LIST_def, transfer, auto simp add:UTYPE_cmlm_def)
-  apply (metis empty_iff list.set(1) list_all_iff)
-  apply (rule injI, transfer, auto simp add:UTYPE_cmlm_def)
+  apply (metis empty_iff list.set(1))
+  apply (rule injI, simp add:ListType_cmlm_def, transfer, auto simp add:UTYPE_cmlm_def)
 done
 end
+
+lemma MkCmlVal_defined_elim [elim!]: 
+  "\<lbrakk> \<D>\<^sub>v (MkCmlVal x); \<And> t. \<lbrakk> \<D> x; x :\<^sub>v t \<rbrakk> \<Longrightarrow> P \<rbrakk> \<Longrightarrow> P"
+  apply (simp add: value_defined_cmlm_def type_rel_cmlm_def)
+  apply (transfer)
+  apply (auto simp add:UTYPE_cmlm_def)
+done
+
+lemma MkCmlVal_type_rel_transfer [simp]: "MkCmlVal x : MkCmlTyp t \<longleftrightarrow> x :\<^sub>v t"
+  by (simp add: type_rel_cmlm_def)
+
+lemma MkCmlTyp_type_rel_elim [elim!]: 
+  "\<lbrakk> x : MkCmlTyp t; \<And> v. \<lbrakk> x = MkCmlVal v; v :\<^sub>v t \<rbrakk> \<Longrightarrow> P \<rbrakk> \<Longrightarrow> P"
+  apply (simp add: type_rel_cmlm_def)
+  apply (transfer)
+  apply (auto simp add: VALUE_cmlm_def)
+done
 
 subsection {* Set Sort instantiation *}
 
 instantiation cmlm :: SET_SORT
 begin
 
-lift_definition MkSet_cmlm :: "cmlm utype \<Rightarrow> cmlm uval bset \<Rightarrow> cmlm uval" is
-"\<lambda> a xs. MkCmlv (SetD (DestCmlt a) (bset_image DestCmlv xs))" by (simp add:UTYPE_cmlm_def VALUE_cmlm_def)
+definition MkSet_cmlm :: "cmlm utype \<Rightarrow> cmlm uval bset \<Rightarrow> cmlm uval" where
+"MkSet a xs = MkCmlVal (SetD (DestCmlTyp a) (bset_image DestCmlVal xs))"
 
-lift_definition DestSet_cmlm :: "cmlm uval \<Rightarrow> cmlm uval bset" is
-"\<lambda> x. bset_image MkCmlv (ProjSetD (DestCmlv x))" 
-  by (auto simp add:VALUE_cmlm_def pred_bset_def bset_image.rep_eq)
+definition DestSet_cmlm :: "cmlm uval \<Rightarrow> cmlm uval bset" where
+"DestSet x = bset_image MkCmlVal (ProjSetD (DestCmlVal x))" 
 
-lift_definition SetType_cmlm :: "cmlm utype \<Rightarrow> cmlm utype" is
-"\<lambda> a. MkCmlt (SetT (DestCmlt a))" by (simp add:UTYPE_cmlm_def)
+definition SetType_cmlm :: "cmlm utype \<Rightarrow> cmlm utype" where
+"SetType a = MkCmlTyp (SetT (DestCmlTyp a))"
 
-instance
-  sorry
+lemma WT_SET_alt_def: 
+  "WT_SET a = {A. \<forall> x\<in>\<^sub>bA. x : a \<and> \<D> (DestCmlVal x)}"
+  by (auto simp add: WT_SET_def value_defined_cmlm_alt_def)
+  
+instance proof (intro_classes, unfold_locales)
+  fix A :: "cmlm uval bset" and t :: "cmlm utype"
+  show "\<D>\<^sub>v (MkSet t A) \<longleftrightarrow> (A \<in> WT_SET t)"
+  proof -
+    have 1:"\<D>\<^sub>v (MkSet t A) \<Longrightarrow> (A \<in> WT_SET t)"
+      apply (clarsimp simp add: WT_SET_alt_def)
+      apply (simp add: value_defined_cmlm_alt_def)
+      apply (auto elim!: SetD_type_cases simp add: value_defined_cmlm_alt_def MkSet_cmlm_def type_rel_cmlm_def)
+      apply (drule sym)
+      apply (simp only: DestBSet_inject)
+      apply (drule_tac x="DestCmlVal x" in spec)
+      apply (simp add:bset_image.rep_eq)
+      apply (metis bset.set_map imageI)
+    done
+    have  2:"(A \<in> WT_SET t) \<Longrightarrow> \<D>\<^sub>v (MkSet t A)"
+      apply (auto simp add: WT_SET_def value_defined_cmlm_alt_def MkSet_cmlm_def bset_image.rep_eq)
+      apply (rule_tac x="MkCmlTyp (SetT (DestCmlTyp t))" in exI)
+      apply (auto simp add:bset_image.rep_eq type_rel_cmlm_def)
+    done
+    from 1 2 show ?thesis ..
+  qed
+next
+  fix A :: "cmlm uval bset" and t :: "cmlm utype"
+  show "A \<in> WT_SET t \<Longrightarrow> MkSet t A : SetType t"
+    apply (auto simp add: WT_SET_alt_def MkSet_cmlm_def SetType_cmlm_def bset_image.rep_eq)
+    apply (simp add:type_rel_cmlm_def)
+  done
+next
+  fix A :: "cmlm uval bset" and t :: "cmlm utype"
+  show "A \<in> WT_SET t \<Longrightarrow> DestSet (MkSet t A) = A"
+    apply (auto simp add: WT_SET_alt_def MkSet_cmlm_def DestSet_cmlm_def SetType_cmlm_def bset_image.rep_eq)
+    apply (rename_tac y)
+    apply (drule_tac x="y" in spec, auto)
+    apply (metis MkCmlTyp_inv MkCmlTyp_type_rel_elim MkCmlVal_inv type_rel_cmlm_def)
+    apply (rename_tac y)
+    apply (drule_tac x="y" in spec, auto)
+    apply (metis DestCmlType_dest MkCmlTyp_type_rel_elim MkCmlVal_inv imageI)
+  done
+next
+  fix A :: "cmlm uval" and t :: "cmlm utype"
+  show "A :! SetType t \<Longrightarrow> MkSet t (DestSet A) = A"
+    by (auto elim!:SetT_type_cases dest!:value_defined_cmlm_dest intro:DestCmlVal_inject 
+             simp add: type_rel_cmlm_def MkSet_cmlm_def DestSet_cmlm_def SetType_cmlm_def)
+next
+  fix t :: "cmlm utype"
+  show "WT_SET t \<noteq> {}"
+    apply (auto simp add: WT_SET_alt_def)
+    apply (rule_tac x="{}\<^sub>b" in exI)
+    apply (simp)
+  done
+next
+  show "inj (SetType :: cmlm utype \<Rightarrow> cmlm utype)"
+    apply (rule injI)
+    apply (simp add:SetType_cmlm_def)
+    apply (metis DestCmlType_dest DestCmlt.simps MkCmlTyp.rep_eq cmlt.inject(1))
+  done
+qed
 
 end
+
+definition EventD :: "cmlm event \<Rightarrow> cmlv" where
+"EventD e = EvD (uchan_name (EventChan e)) 
+                (DestCmlTyp (uchan_type (EventChan e)))
+                (DestCmlVal (EventValue e))"
+
+primrec ProjEventD :: "cmlv \<Rightarrow> cmlm event" where
+"ProjEventD (EvD n t v) = Event n (MkCmlTyp t) (MkCmlVal v)"
+
+lemma EventD_type [typing,intro]:
+  "EventD e :\<^sub>v EventT"
+  apply (case_tac e)
+  apply (auto simp add:EventD_def type_rel_cmlm_def)
+done
+
+lemma EventD_defined [simp]:
+  "\<D> (EventD e)"
+  by (simp add:EventD_def)
+
+lemma EventI_inv [simp]:
+  "ProjEventD (EventD e) = e"
+  apply (simp add:EventD_def)
+  apply (metis DestCmlType_dest DestCmlVal_inject EventChan.rep_eq EventValue.rep_eq MkCmlVal_inv RepEvent_inverse RepUChan_inverse prod.swap_def surj_pair swap_simp)
+done
+
+
+instantiation cmlm :: EVENT_SORT
+begin
+
+definition MkEvent_cmlm :: "cmlm event \<Rightarrow> cmlm uval" where
+"MkEvent e = MkCmlVal (EventD e)"
+
+definition DestEvent_cmlm :: "cmlm uval \<Rightarrow> cmlm event" where
+"DestEvent_cmlm e = ProjEventD (DestCmlVal e)"
+
+definition EventType_cmlm :: "cmlm utype" where
+"EventType_cmlm = MkCmlTyp EventT"
+
+instance
+  apply (intro_classes, unfold_locales, auto simp add:MkEvent_cmlm_def 
+                        EventType_cmlm_def DestEvent_cmlm_def value_defined_cmlm_def)
+  apply (rule_tac x="MkCmlTyp EventT" in exI, force)
+  apply (simp add:EventD_def)
+  apply (metis DestCmlType_dest monotype_def type_rel_cmlm_def vbasic_type_rel_uniq)
+done
+
+end
+
+instance cmlm :: REACTIVE_SORT ..
 
 end
