theories/models/utp_cml_new/utp_cml_process.thy
@@ -1,0 +1,329 @@
+(******************************************************************************)
+(* Project: CML model for Isabelle/UTP                                        *)
+(* File: utp_cml_process.thy                                                  *)
+(* Author: Simon Foster, University of York (UK)                              *)
+(******************************************************************************)
+
+header {* CML processes *}
+
+theory utp_cml_process
+imports 
+  utp_cml_stmt
+begin
+
+text {* Add a simple syntax translator for main actions in CML processes. The ML
+        function simply appends .MainAction. *}
+
+syntax
+  "_cml_proc_ref_0" :: "id \<Rightarrow> n_upred" ("@_'(')" [10] 10)
+  "_cml_proc_ref_1" :: "id \<Rightarrow> n_pexpr \<Rightarrow> n_upred" ("@_'(_')" [10,10] 10)
+  "_cml_proc_ref_2" :: "id \<Rightarrow> n_pexpr \<Rightarrow> n_pexpr \<Rightarrow> n_upred" ("@_'(_,/ _')" [10,10,10] 10)
+  "_cml_proc_ref_3" :: "id \<Rightarrow> n_pexpr \<Rightarrow> n_pexpr \<Rightarrow> n_pexpr \<Rightarrow> n_upred" ("@_'(_,/ _,/ _')" [10,10,10,10] 10)
+
+parse_ast_translation {*
+let
+  fun cml_proc_ref_tr_0 [Ast.Variable full_name] =
+    Ast.Variable (full_name ^ ".MainAction")
+  | cml_proc_ref_tr_0 e = raise Match;
+  fun cml_proc_ref_tr_1 [Ast.Variable full_name, p] =
+    Ast.Appl [Ast.Constant @{const_syntax Op1PP}, Ast.Variable (full_name ^ ".MainAction"), p]
+  | cml_proc_ref_tr_1 e = raise Match;
+  fun cml_proc_ref_tr_2 [Ast.Variable full_name, p, q] =
+    Ast.Appl [Ast.Constant @{const_syntax Op2PP}, Ast.Variable (full_name ^ ".MainAction"), p, q]
+  | cml_proc_ref_tr_2 e = raise Match;
+  fun cml_proc_ref_tr_3 [Ast.Variable full_name, p, q, r] =
+    Ast.Appl [Ast.Constant @{const_syntax Op3PP}, Ast.Variable (full_name ^ ".MainAction"), p, q, r]
+  | cml_proc_ref_tr_3 e = raise Match;
+in
+  [(@{syntax_const "_cml_proc_ref_0"}, K cml_proc_ref_tr_0)
+  ,(@{syntax_const "_cml_proc_ref_1"}, K cml_proc_ref_tr_1)
+  ,(@{syntax_const "_cml_proc_ref_2"}, K cml_proc_ref_tr_2)
+  ,(@{syntax_const "_cml_proc_ref_3"}, K cml_proc_ref_tr_3)]
+end
+*}
+
+definition ForLoopSetD :: "'a bset cmle \<Rightarrow> ('a option \<Rightarrow> cmlp) \<Rightarrow> cmlp" where
+"ForLoopSetD xs F = undefined"
+
+definition ParallelD :: 
+  "cmlp \<Rightarrow> cmlev bset \<Rightarrow> cmlp \<Rightarrow> cmlp" where
+"ParallelD p cs q = ParallelCSP p (LitPE (Abs_USET cs)) q"
+
+definition ReplSeqSetD ::
+  "'a bset cmle \<Rightarrow> ('a \<Rightarrow> cmlp) \<Rightarrow> cmlp" where
+"ReplSeqSetD = undefined"
+
+definition ReplIntSetD ::
+  "'a bset cmle \<Rightarrow> ('a \<Rightarrow> cmlp) \<Rightarrow> cmlp" where
+"ReplIntSetD = undefined"
+
+definition ReplExtSetD ::
+  "'a bset cmle \<Rightarrow> ('a \<Rightarrow> cmlp) \<Rightarrow> cmlp" where
+"ReplExtSetD = undefined"
+
+definition ReplExtTyD ::
+  "'a set \<Rightarrow> ('a \<Rightarrow> cmlp) \<Rightarrow> cmlp" where
+"ReplExtTyD = undefined"
+
+definition ReplParSetD ::
+  "'a bset cmle \<Rightarrow> ('a \<Rightarrow> cmlp) \<Rightarrow> cmlp" where
+"ReplParSetD = undefined"
+
+definition ReplAlphaParSetD ::
+  "'a bset cmle \<Rightarrow> cmlev set \<Rightarrow> ('a \<Rightarrow> cmlp) \<Rightarrow> cmlp" where
+"ReplAlphaParSetD = undefined"
+
+definition ReplInlvSetD ::
+  "'a bset cmle \<Rightarrow> ('a \<Rightarrow> cmlp) \<Rightarrow> cmlp" where
+"ReplInlvSetD = undefined"
+
+definition HideD ::
+  "cmlp \<Rightarrow> cmlev set \<Rightarrow> cmlp" where
+"HideD p cs = undefined"
+
+definition InterruptD :: "cmlp \<Rightarrow> cmlp \<Rightarrow> cmlp" where
+"InterruptD p q = undefined"
+
+definition TimeoutD :: "cmlp \<Rightarrow> real cmle \<Rightarrow> cmlp \<Rightarrow> cmlp" where
+"TimeoutD p n q = undefined"
+
+definition UTimeoutD :: "cmlp \<Rightarrow> cmlp \<Rightarrow> cmlp" where
+"UTimeoutD p q = undefined"
+
+definition WaitD :: "real cmle \<Rightarrow> cmlp" where
+"WaitD n = undefined"
+
+abbreviation MkChanD :: "string \<Rightarrow> 'a set \<Rightarrow> ('a option) chan" where
+"MkChanD n xs \<equiv> AbsChan (bName n, TYPE('a option))"
+
+
+(* FIXME: Execution of CML operations needs to take care of undefinedness *)
+
+(* FIXME: Surely these can all be unified into a single thing ... *)
+
+definition Exec0D :: "cmlp \<Rightarrow> cmlp" where
+"Exec0D p = p"
+
+lift_definition Exec1D :: 
+  "('a option \<Rightarrow> cmlp) \<Rightarrow> 'a cmle \<Rightarrow> cmlp" 
+  is "\<lambda> P e. {b :: cmlm binding. b \<in> P (e b)}" .
+
+lift_definition Exec2D :: 
+  "('a option \<Rightarrow> 'b option \<Rightarrow> cmlp) \<Rightarrow> 'a cmle \<Rightarrow> 'b cmle \<Rightarrow> cmlp" 
+  is "\<lambda> P e f. {b :: cmlm binding. b \<in> P (e b) (f b)}" .
+
+lift_definition Exec3D :: 
+  "('a option \<Rightarrow> 'b option \<Rightarrow> 'c option \<Rightarrow> cmlp) 
+   \<Rightarrow> 'a cmle \<Rightarrow> 'b cmle \<Rightarrow> 'c cmle \<Rightarrow> cmlp" 
+  is "\<lambda> P e f g. {b :: cmlm binding. b \<in> P (e b) (f b) (g b)}" .
+
+lift_definition Exec4D :: 
+  "('a option \<Rightarrow> 'b option \<Rightarrow> 'c option \<Rightarrow> 'd option \<Rightarrow> cmlp) 
+   \<Rightarrow> 'a cmle \<Rightarrow> 'b cmle \<Rightarrow> 'c cmle \<Rightarrow> 'd cmle \<Rightarrow> cmlp" 
+  is "\<lambda> P e f g h. {b :: cmlm binding. b \<in> P (e b) (f b) (g b) (h b)}" .
+
+lift_definition Exec5D :: 
+  "('a option \<Rightarrow> 'b option \<Rightarrow> 'c option \<Rightarrow> 'd option \<Rightarrow> 'e option \<Rightarrow> cmlp) 
+   \<Rightarrow> 'a cmle \<Rightarrow> 'b cmle \<Rightarrow> 'c cmle \<Rightarrow> 'd cmle \<Rightarrow> 'e cmle \<Rightarrow> cmlp" 
+  is "\<lambda> P e f g h i. {b :: cmlm binding. b \<in> P (e b) (f b) (g b) (h b) (i b)}" .
+
+lift_definition Exec6D :: 
+  "('a option \<Rightarrow> 'b option \<Rightarrow> 'c option \<Rightarrow> 'd option \<Rightarrow> 'e option \<Rightarrow> 'f option \<Rightarrow> cmlp) 
+   \<Rightarrow> 'a cmle \<Rightarrow> 'b cmle \<Rightarrow> 'c cmle \<Rightarrow> 'd cmle \<Rightarrow> 'e cmle \<Rightarrow> 'f cmle \<Rightarrow> cmlp" 
+  is "\<lambda> P e f g h i j. {b :: cmlm binding. b \<in> P (e b) (f b) (g b) (h b) (i b) (j b)}" .
+
+definition CmlAbsP :: "'a set \<Rightarrow> ('a \<Rightarrow> 'b::type) \<Rightarrow> ('a \<Rightarrow> 'b)" where
+"CmlAbsP A P = P"
+
+(* We remove the standard definition of prefix and add one specific for CML *)
+
+no_syntax
+  "_upred_prefixed"  :: "n_pexpr \<Rightarrow> n_upred \<Rightarrow> n_upred" ("_ -> _")
+  "_upred_input"     :: "'a chan \<Rightarrow> pttrn \<Rightarrow> n_upred \<Rightarrow> n_upred" ("_?_ -> _")
+  "_upred_output"    :: "'a chan \<Rightarrow> n_pexpr \<Rightarrow> n_upred \<Rightarrow> n_upred" ("_!_ -> _")
+  "_upred_event"     :: "'a chan \<Rightarrow> n_pexpr \<Rightarrow> n_upred \<Rightarrow> n_upred" ("_._ -> _")
+  "_upred_PrefixSkipCSP" :: "n_pexpr \<Rightarrow> n_upred" ("@_")
+
+no_syntax (xsymbols)
+  "_upred_prefixed"  :: "n_pexpr \<Rightarrow> n_upred \<Rightarrow> n_upred" ("_ \<rightarrow> _")
+
+nonterminal n_chanset and n_chan and n_chans and n_comm and n_comms
+
+term "SUP x:A. PrefixCSP x p"
+
+syntax
+  "_n_chan_ev"       :: "idt => idt => n_chan"  ("_@_")
+  "_n_chan_ch"       :: "idt => n_chan" ("_")
+  "_n_chan"          :: "n_chan => n_chans" ("_")
+  "_n_chans"         :: "[n_chan, n_chans] => n_chans" ("_,/ _")
+  "_n_comm_dot"      :: "n_pexpr \<Rightarrow> n_comm \<Rightarrow> n_comm" (".'(_')_")
+  "_n_chanset_id"    :: "idt \<Rightarrow> n_chanset" ("_")
+  "_n_chanset_enum"  :: "n_chans \<Rightarrow> n_chanset" ("{|(_)|}")
+(*  "_n_chanset_comp"  :: "n_comm \<Rightarrow> vbinds \<Rightarrow> n_chanset" ("{| _ | _ |}") *)
+  "_n_chanset_union" :: "n_chanset \<Rightarrow> n_chanset \<Rightarrow> n_chanset" (infixl "union" 65)
+  "_n_chanset_inter" :: "n_chanset \<Rightarrow> n_chanset \<Rightarrow> n_chanset" (infixl "inter" 70)
+  "_n_chanset_diff"  :: "n_chanset \<Rightarrow> n_chanset \<Rightarrow> n_chanset" (infixl "\\" 70)
+  "_n_chanset_val_enum" :: "n_chans \<Rightarrow> logic" ("{|(_)|}")
+
+ML {* absdummy dummyT *}
+
+translations
+  "_n_chan_ev c v"   => "CONST insert (CONST PEvent c v) {}"
+  "_n_chan_ch c"     => "CONST EventSet {c\<down>}"
+  "_n_chan cs"       => "cs"
+  "_n_chans cs1 cs2" => "cs1 \<union> cs2"
+  "_n_chanset_id x"    => "x"
+  "_n_chanset_enum cs" => "cs"
+  "_n_chanset_union cs1 cs2" => "cs1 \<union> cs2"
+  "_n_chanset_inter cs1 cs2" => "cs1 \<inter> cs2"
+  "_n_chanset_diff  cs1 cs2" => "cs1 - cs2"
+  "_n_chanset_val_enum cs" => "cs"
+
+syntax
+(*  "_n_upred_cml_prefix" :: "unit option CHAN \<Rightarrow> n_upred \<Rightarrow> n_upred" ("_ -> _") *)
+  "_n_upred_parcml"     :: "n_upred \<Rightarrow> n_chanset \<Rightarrow> n_upred \<Rightarrow> n_upred" (infixl "[|_|]" 50)
+  "_n_upred_aseqsetcml" :: "idt \<Rightarrow> n_pexpr \<Rightarrow> n_upred \<Rightarrow> n_upred" ("; _ in @set _ @ _" [0,0,10] 10)
+  "_n_upred_aextsetcml" :: "idt \<Rightarrow> n_pexpr \<Rightarrow> n_upred \<Rightarrow> n_upred" ("[] _ in @set _ @ _" [0,0,10] 10)
+  "_n_upred_aexttycml"  :: "idt \<Rightarrow> vty \<Rightarrow> n_upred \<Rightarrow> n_upred" ("[] _ : _ @ _" [0,0,10] 10)
+  "_n_upred_aintsetcml" :: "idt \<Rightarrow> n_pexpr \<Rightarrow> n_upred \<Rightarrow> n_upred" ("|~| _ in @set _ @ _" [0,0,10] 10)
+  "_n_upred_aparsetcml"   :: "idt \<Rightarrow> n_pexpr \<Rightarrow> n_upred \<Rightarrow> n_upred" ("|| _ in @set _ @ _" [0,0,10] 10)
+  "_n_upred_aparsetevcml" :: "idt \<Rightarrow> n_pexpr \<Rightarrow> n_chanset \<Rightarrow> n_upred \<Rightarrow> n_upred" ("|| _ in @set _ @ [_] _" [0,0,0,10] 10)
+  "_n_upred_ainlvsetcml" :: "idt \<Rightarrow> n_pexpr \<Rightarrow> n_upred \<Rightarrow> n_upred" ("||| _ in @set _ @ _" [0,0,10] 10)
+  "_n_upred_hidecml"    :: "n_upred \<Rightarrow> n_chanset \<Rightarrow> n_upred" (infixl "\\" 60)
+  "_n_upred_intrptcml"  :: "n_upred \<Rightarrow> n_upred \<Rightarrow> n_upred" (infixl "'/-\\" 50)
+  "_n_upred_timeoutcml" :: "n_upred \<Rightarrow> n_pexpr \<Rightarrow> n_upred \<Rightarrow> n_upred" (infixl "[_>" 50)
+  "_n_upred_utimeoutcml" :: "n_upred \<Rightarrow> n_upred \<Rightarrow> n_upred" (infixl "[>" 50)
+  "_n_upred_waitcml"    :: "n_pexpr \<Rightarrow> n_upred" ("WAIT _")
+  "_n_upred_cml_exec0"  :: "idt \<Rightarrow> n_upred" ("_'(')")
+  "_n_upred_cml_exec1"  :: "idt \<Rightarrow> n_pexpr \<Rightarrow> n_upred" ("_'(_')")
+  "_n_upred_cml_exec2"  :: "idt \<Rightarrow> n_pexpr \<Rightarrow> n_pexpr \<Rightarrow> n_upred" ("_'(_, _')")
+  "_n_upred_cml_exec3"  :: "idt \<Rightarrow> n_pexpr \<Rightarrow> n_pexpr \<Rightarrow> n_pexpr \<Rightarrow> n_upred" ("_'(_, _, _')")
+  "_n_upred_cml_exec4"  :: "idt \<Rightarrow> n_pexpr \<Rightarrow> n_pexpr \<Rightarrow> n_pexpr \<Rightarrow> n_pexpr \<Rightarrow> n_upred" ("_'(_, _, _, _')")
+  "_n_upred_cml_exec5"  :: "idt \<Rightarrow> n_pexpr \<Rightarrow> n_pexpr \<Rightarrow> n_pexpr \<Rightarrow> n_pexpr \<Rightarrow> n_pexpr \<Rightarrow> n_upred" ("_'(_, _, _, _, _')")
+  "_n_upred_cml_exec6"  :: "idt \<Rightarrow> n_pexpr \<Rightarrow> n_pexpr \<Rightarrow> n_pexpr \<Rightarrow> n_pexpr \<Rightarrow> n_pexpr \<Rightarrow> n_pexpr \<Rightarrow> n_upred" ("_'(_, _, _, _, _, _')")
+  "_cml_proc_abs"       :: "vtype_binds \<Rightarrow> n_upred \<Rightarrow> n_upred" ("_ @ _" [30,30] 30)
+
+term "case_prod"
+
+translations
+  "_n_upred_parcml p vs q"        == "CONST ParallelD p vs q"
+  "_n_upred_aseqsetcml x vs p"    == "CONST ReplSeqSetD vs (\<lambda> x. p)"
+  "_n_upred_aintsetcml x vs p"    == "CONST ReplIntSetD vs (\<lambda> x. p)"
+  "_n_upred_aextsetcml x vs p"    == "CONST ReplExtSetD vs (\<lambda> x. p)"
+  "_n_upred_aexttycml x vs p"     == "CONST ReplExtTyD vs (\<lambda> x. p)"
+  "_n_upred_aparsetcml x vs p"    == "CONST ReplParSetD vs (\<lambda> x. p)" 
+  "_n_upred_aparsetevcml x vs es p" == "CONST ReplAlphaParSetD vs es (\<lambda> x. p)"
+  "_n_upred_ainlvsetcml x vs p"   == "CONST ReplInlvSetD vs (\<lambda> x. p)"
+  "_n_upred_hidecml p cs"         == "CONST HideD p cs"
+  "_n_upred_intrptcml p q"        == "CONST InterruptD p q"
+  "_n_upred_timeoutcml p n q"     == "CONST TimeoutD p n q"
+  "_n_upred_utimeoutcml p q"      == "CONST TimeoutD p q"
+  "_n_upred_waitcml n"            == "CONST WaitD n"
+(*  "_n_upred_cml_prefix n p"       == "CONST CommD n p" *)
+  "_n_upred_cml_exec0 s"          == "CONST RH (CONST Exec0D s)"
+  "_n_upred_cml_exec1 f s"        == "CONST RH (CONST Exec1D f s)"
+  "_n_upred_cml_exec2 v1 v2 s"    == "CONST RH (CONST Exec2D v1 v2 s)"
+  "_n_upred_cml_exec3 v1 v2 v3 s" == "CONST RH (CONST Exec3D v1 v2 v3 s)"
+  "_n_upred_cml_exec3 v1 v2 v3 v4 s" == "CONST RH (CONST Exec3D v1 v2 v3 v4 s)"
+  "_n_upred_cml_exec3 v1 v2 v3 v4 v5 s" == "CONST RH (CONST Exec3D v1 v2 v3 v4 v5 s)"
+  "_n_upred_cml_exec3 v1 v2 v3 v4 v5 v6 s" == "CONST RH (CONST Exec3D v1 v2 v3 v4 v5 v6 s)"
+  (* Parse rules for parametric actions *)
+  "_cml_proc_abs (_vtype_bind (_vtybind (_vidts x xs) A)) P" 
+    => "CONST case_prod (CONST CmlAbsP A (\<lambda> x . (_cml_proc_abs (_vtype_bind (_vtybind xs A)) P)))" 
+  "_cml_proc_abs (_vtype_bind (_vtybind (_vidt x) A)) P"   => "CONST CmlAbsP A (\<lambda> x. (P :: cmlp))"
+  "_cml_proc_abs (_vtype_binds (_vtybind (_vidts x xs) A) bs) P" 
+    => "CONST case_prod (CONST CmlAbsP A (\<lambda> x . (_cml_proc_abs (_vtype_binds (_vtybind xs A) bs) P)))"
+  "_cml_proc_abs (_vtype_binds (_vtybind (_vidt x) A) bs) P"  
+    => "CONST case_prod (CONST CmlAbsP A (\<lambda> x. _cml_proc_abs bs P))"
+  (* Print rules for parametric actions *)
+(*
+  "_cml_proc_abs (_vtype_bind (_vtybind (_vidt x) A)) P" <= "CONST CmlAbsP A (\<lambda> x . P)"
+  "_cml_proc_abs (_vtype_bind (_vtybind (_vidt x) A)) P" <= "CONST CmlAbsP A (\<lambda> x . P)"
+*)
+
+term "`(i:@bool,j,k:@nat,l:@bool @ P)`"
+
+term "`([] i in @set {1,2,3} @ P) ; Q`"
+term "`|| i in @set {1,2,3} @ P [(&i)> Q`"
+term "`||| i in @set {1,2,3} @ (P [(&i)> Q)`"
+term "`; i in @set {1,2,3} @ (P [(&i)> Q)`"
+term "`[] i in @set {1,2,3} @ (P [(&i)> Q)`"
+term "`[] i : @nat @ (P [(&i)> Q)`"
+term "`|| i in @set {1,2,3} @ [{|v|}] (P [(&i)> Q)`"
+(* term "`P [|{|x,y,z|}|] Q`" *)
+term "`P \\ {|x,y,z|}`"
+term "`P \\ {|x,y|} union {|z|}`"
+term "`P \\ xs`"
+term "`P /-\\ Q`"
+term "`P [(5)> Q`"
+term "`P [> Q`"
+term "`WAIT $x ; WAIT $y`"
+term "`f()`"
+term "`P<1>`"
+
+text {* CML event prefix syntax *}
+
+no_syntax
+  "_n_upred_prefixed"      :: "n_pexpr \<Rightarrow> n_upred \<Rightarrow> n_upred" ("_ -> _")
+  "_n_upred_index"         :: "('b \<Rightarrow> 'a upred) \<Rightarrow> 'b \<Rightarrow> n_upred" ("_<_>" 50)
+  "_n_upred_PrefixSkipCSP" :: "n_pexpr \<Rightarrow> n_upred" ("@_")
+
+syntax
+  "_n_comm_nil"      :: "n_comm" ("")
+  "_n_comm_inp"      :: "idt \<Rightarrow> n_comm \<Rightarrow> n_comm" ("?'(_')_")
+  "_n_comm_outp"     :: "n_pexpr \<Rightarrow> n_comm \<Rightarrow> n_comm" ("!'(_')_")
+  "_cml_comm"        :: "idt \<Rightarrow> n_comm \<Rightarrow> n_upred \<Rightarrow> n_upred" ("__ -> _" [20,50,50] 50)
+  "_cml_comm_body"   :: "idt \<Rightarrow> n_comm \<Rightarrow> n_upred \<Rightarrow> n_upred"
+  "_cml_comm_bind"   :: "n_comm \<Rightarrow> idt \<Rightarrow> n_comm \<Rightarrow> n_upred \<Rightarrow> n_upred \<Rightarrow> logic"
+  "_cml_comm_prod"   :: "n_comm \<Rightarrow> logic"
+
+(*
+translations
+  "_cml_comm c _n_comm_nil (_n_upred_SkipCSP)" <= "CONST Output c SKIP"
+*)
+
+text {* This rather complex set of translations performs two passes over a list 
+        of channel variables:
+        - in the first pass, a big external choice is entered for each input, and all
+          other kinds are ignored
+        - in the second pass, each variable is inserted into a tuple and then composed
+          with the channel. 
+       FIXME: Currently we don't insert correct type data for the external choice,
+              this should be extracted somehow from the channel.
+*}
+
+translations
+  "_cml_comm_prod (_n_comm_nil)" => "CONST UnitD"
+  "_cml_comm_prod (_n_comm_dot v _n_comm_nil)" => "v"
+  "_cml_comm_prod (_n_comm_dot v vs)"  => "CONST vexpr_prod v (_cml_comm_prod vs)"
+  "_cml_comm_prod (_n_comm_inp v _n_comm_nil)" => "(CONST LitD v)"
+  "_cml_comm_prod (_n_comm_inp x vs)"  => "CONST vexpr_prod (CONST LitD x) (_cml_comm_prod vs)"
+  "_cml_comm_prod (_n_comm_outp v _n_comm_nil)" => "v"
+  "_cml_comm_prod (_n_comm_outp v vs)" => "CONST vexpr_prod v (_cml_comm_prod vs)"
+  "_cml_comm_bind (_n_comm_nil) c v p" => "_cml_comm_body c v p"
+  "_cml_comm_bind (_n_comm_dot x _n_comm_nil) c v p" => "_cml_comm_body c v p"
+  "_cml_comm_bind (_n_comm_dot x vs) c v p"  => "_cml_comm_bind vs c v p"
+  "_cml_comm_bind (_n_comm_inp x _n_comm_nil) c v p" 
+      => "CONST ReplExtTyD CONST UNIV (\<lambda> x. (_cml_comm_body c v p))"
+  "_cml_comm_bind (_n_comm_inp x vs) c v p"  
+      => "CONST ReplExtTyD CONST UNIV (\<lambda> x. (_cml_comm_bind vs c v p))"
+  "_cml_comm_bind (_n_comm_outp x _n_comm_nil) c v p" => "_cml_comm_body c v p"
+  "_cml_comm_bind (_n_comm_outp x vs) c v p"  => "_cml_comm_bind vs c v p"
+  "_cml_comm_body c v p"               => "CONST OutputCSP c (_cml_comm_prod v) p"
+  "_cml_comm c v p"                    => "_cml_comm_bind v c v p"
+
+(* Add pretty printing for 1-4 communications *)
+
+translations
+  "_cml_comm c (_n_comm_dot u (_n_comm_dot v (_n_comm_dot w (_n_comm_dot x _n_comm_nil)))) p"
+    <= "CONST OutputCSP c (CONST vexpr_prod u (CONST vexpr_prod v (CONST vexpr_prod w x))) p"
+  "_cml_comm c (_n_comm_dot u (_n_comm_dot v (_n_comm_dot w _n_comm_nil))) p"
+    <= "CONST OutputCSP c (CONST vexpr_prod u (CONST vexpr_prod v w)) p"
+  "_cml_comm c (_n_comm_dot u (_n_comm_dot v _n_comm_nil)) p" 
+    <= "CONST OutputCSP c (CONST vexpr_prod u v) p"
+  "_cml_comm c (_n_comm_nil) p"
+  <= "CONST OutputCSP c (CONST UnitD) p"
+  "_cml_comm c (_n_comm_dot u _n_comm_nil) p"
+  <= "CONST OutputCSP c u p"
+
+end
