theories/models/utp_cml_new/utp_cml_records.thy
@@ -1,0 +1,261 @@
+(******************************************************************************)
+(* Project: CML model for Isabelle/UTP                                        *)
+(* File: utp_cml_records.thy                                                  *)
+(* Author: Simon Foster, University of York (UK)                              *)
+(******************************************************************************)
+
+header {* CML records *}
+
+theory utp_cml_records
+imports 
+  utp_cml_expr
+  utp_cml_functions
+  utp_cml_types
+begin
+
+default_sort type
+
+text {* CML records are formalised as tagged types, unit types which carry a string. *}
+
+class tag =
+  fixes tagName :: "'a \<Rightarrow> string"
+  assumes tagUnit: "(x::'a) = y"
+begin
+
+definition tag :: "'a" where
+"tag = (THE x. True)"
+
+end
+
+text {* A CML field over a given tag, field type and record type consists of
+        an accessor function and CML type. The CML type must not be empty. *}
+
+typedef ('t::tag, 'a::cmlv, 'r) field =
+  "UNIV :: (('r \<Rightarrow> 'a) * 'a set) set"
+  by (auto)
+
+declare Abs_field_inverse [simp]
+
+setup_lifting type_definition_field
+
+lift_definition FieldProj :: 
+  "('t::tag, 'a::cmlv, 'r) field \<Rightarrow> ('r \<Rightarrow> 'a)" is "fst" ..
+
+declare FieldProj.rep_eq [simp]
+
+lift_definition FieldType ::
+  "('t::tag, 'a::cmlv, 'r) field \<Rightarrow> 'a set" is "snd" ..
+
+declare FieldType.rep_eq [simp]
+
+(* declare MkField_def [eval,evalp] *)
+
+typedef ('t, 'a, 'r) tagged = "UNIV :: 'a set set"
+  by (auto)
+
+declare Rep_tagged [simp]
+declare Abs_tagged_inverse [simp]
+declare Abs_tagged_inject [simp]
+declare Rep_tagged_inverse [simp]
+declare Rep_tagged_inject [simp]
+
+typedef ('t, 'r) rec = "UNIV :: 'r set"
+  by (auto)
+
+declare Rep_rec [simp]
+declare Abs_rec_inverse [simp]
+declare Abs_rec_inject [simp]
+declare Rep_rec_inverse [simp]
+declare Rep_rec_inject [simp]
+
+(* setup_lifting type_definition_rec *)
+
+instantiation rec :: (tag, cmlv) cmlv
+begin
+
+definition Inject_rec :: "('a, 'b) rec \<Rightarrow> cmlv" where
+"Inject_rec r = TagD (tagName (tag :: 'a)) (Inject (Rep_rec r))"
+
+definition Type_rec :: "('a, 'b) rec itself \<Rightarrow> cmlt" where
+"Type_rec rt = TagT (tagName (tag :: 'a)) VTYPE('b)"
+
+instance 
+  apply (intro_classes)
+  apply (auto simp add:Inject_rec_def Type_rec_def Rep_rec_inject image_def)
+  apply (metis Project_Inject Rep_rec_cases UNIV_I)
+done
+end
+
+definition plast_rec :: "('a::type, 'b::type) rec \<Rightarrow> ('a, 'b) rec" where
+"plast_rec = id"
+
+declare plast_rec_def [evalp]
+
+adhoc_overloading
+  plast plast_rec
+
+instantiation rec :: (type, linorder) linorder
+begin
+
+definition less_eq_rec :: "('a, 'b) rec \<Rightarrow> ('a, 'b) rec \<Rightarrow> bool" where
+"r1 \<le> r2 = (Rep_rec r1 \<le> Rep_rec r2)"
+
+definition less_rec :: "('a, 'b) rec \<Rightarrow> ('a, 'b) rec \<Rightarrow> bool" where
+"r1 < r2 = (Rep_rec r1 < Rep_rec r2)"
+
+instance
+  apply (intro_classes)
+  apply (auto simp add:less_eq_rec_def less_rec_def)
+  apply (metis Rep_rec_inject less_le)
+done
+end
+
+definition UnitField :: "('t::tag, 'a::cmlv, 'r) field \<Rightarrow> ('t, 'a, 'r) tagged" where
+"UnitField f = Abs_tagged (FieldType f)"
+
+(* declare UnitField_def [eval,evalp] *)
+
+definition ConsField :: 
+  "('t::tag, 'a::cmlv, 'r) field \<Rightarrow> 
+   ('t, 'b, 'r) tagged \<Rightarrow>  
+   ('t, ('a * 'b), 'r) tagged" where
+"ConsField f t = Abs_tagged (FieldType f \<times> Rep_tagged t)"
+
+(* declare ConsField_def [eval,evalp] *)
+
+definition MkTagRec :: "('t::tag, 'r::cmlv, 'r) tagged \<Rightarrow> 'r \<Rightarrow> ('t, 'r) rec" where
+"MkTagRec t = Abs_rec"
+
+(* declare MkTagRec_def [eval,evalp] *)
+
+definition MkField :: "('t::tag, 'r) rec set \<Rightarrow> ('r \<Rightarrow> 'a) \<Rightarrow> 'a::cmlv set \<Rightarrow> ('t,'a,'r) field" where
+"MkField t f x = Abs_field (f, x)"
+
+definition TermField :: "('t::tag, 'r::cmlv, 's) tagged \<Rightarrow> ('t, 'r) rec set" where
+"TermField t \<equiv> Abs_rec ` Rep_tagged t"
+
+abbreviation FinishField :: "('t::tag, 'r::cmlv, 'r) tagged \<Rightarrow> ('t, 'r) rec set" where
+"FinishField \<equiv> TermField"
+
+definition RecMaximalType :: "'a set \<Rightarrow> 't::tag itself \<Rightarrow> ('t, 'a) rec set"
+where "RecMaximalType xs t = Abs_rec ` xs"
+
+(*
+definition FinishField :: "('t::tag, 'r::vbasic, 'r) tagged \<Rightarrow> ('t, 'r) rec set" where
+"FinishField t \<equiv> MkTagRec t ` Rep_tagged t"
+*)
+
+(* declare FinishField_def [eval,evalp] *)
+
+definition MkRec :: "('t::tag, 'r::cmlv) rec set \<Rightarrow> 'r \<Rightarrow> ('t, 'r) rec cmle" where
+"MkRec t r = LitD (Abs_rec r)"
+
+declare MkRec_def [eval, evalp]
+
+definition SelectRec :: 
+  "('t::tag, 'a::cmlv, 'r) field \<Rightarrow> 
+   ('t, 'r) rec \<Rightarrow> 'a" where
+"SelectRec f r = (fst (Rep_field f)) (Rep_rec r)"
+
+(* declare SelectRec_def [eval,evalp] *)
+
+nonterminal vty_fields and vrec
+
+syntax
+  "_vty_fields"    :: "('t, 'a, 'r) field \<Rightarrow> vty_fields => vty_fields" ("_,/ _")
+  "_vty_field"     :: "('t, 'a, 'r) field \<Rightarrow> vty_fields" ("_")
+  "_vty_record"    :: "vty_fields => vty"    ("[(_)]")
+
+translations
+  "_vty_fields x xs" == "CONST ConsField x xs"
+  "_vty_field x" == "CONST UnitField x"
+  "_vty_record x" == "CONST FinishField x"
+
+lemma Abs_rec_cons_type [simp]:
+  "Abs_rec (x, y) \<in> TermField (ConsField a b)
+   \<longleftrightarrow> (x \<in> FieldType a \<and> Abs_rec y \<in> TermField b)"
+  by (auto simp add:TermField_def MkTagRec_def ConsField_def UnitField_def)
+
+lemma Abs_rec_unit_type [simp]:
+  "Abs_rec x \<in> TermField (UnitField a)
+   \<longleftrightarrow> x \<in> FieldType a"
+  by (auto simp add:TermField_def MkTagRec_def ConsField_def UnitField_def)
+
+lemma [simp]: "Rep_field (MkField t f x) = (f, x)"
+  by (simp add:MkField_def)
+
+lemma SelectRec_simp [simp]:
+  "SelectRec (MkField t f u) (Abs_rec x) = f x"
+  by (simp add:SelectRec_def)
+
+(*
+lemma SelectRec_1_2 [simp]: 
+  "SelectRec (MkField g #[1] t u) (Abs_rec (v1, r)) = v1"
+  by (simp add:SelectRec_def vprod_simps)
+
+lemma SelectRec_2 [simp]: 
+  "SelectRec (MkField g #[2] t u) (Abs_rec (v1, v2, r)) = v2"
+  by (simp add:SelectRec_def vprod_simps)
+
+lemma SelectRec_3 [simp]: 
+  "SelectRec (MkField g #[3] t u) (Abs_rec (v1, v2, v3, r)) = v3"
+  by (simp add:SelectRec_def vprod_simps)
+
+lemma SelectRec_4 [simp]: 
+  "SelectRec (MkField g #[4] t u) (Abs_rec (v1, v2, v3, v4, r)) = v4"
+  by (simp add:SelectRec_def vprod_simps)
+
+lemma SelectRec_5 [simp]: 
+  "SelectRec (MkField g #[5] t u) (Abs_rec (v1, v2, v3, v4, v5, r)) = v5"
+  by (simp add:SelectRec_def vprod_simps)
+
+lemma SelectRec_6 [simp]: 
+  "SelectRec (MkField g #[6] t u) (Abs_rec (v1, v2, v3, v4, v5, v6, r)) = v6"
+  by (simp add:SelectRec_def vprod_simps)
+
+lemma SelectRec_7 [simp]: 
+  "SelectRec (MkField g #[7] t u) (Abs_rec (v1, v2, v3, v4, v5, v6, v7, r)) = v7"
+  by (simp add:SelectRec_def vprod_simps)
+
+lemma SelectRec_8 [simp]: 
+  "SelectRec (MkField g #[8] t u) (Abs_rec (v1, v2, v3, v4, v5, v6, v7, v8, r)) = v8"
+  by (simp add:SelectRec_def vprod_simps)
+*)
+
+(*
+typedef MyRec_Tag = "{True}" by auto
+instantiation MyRec_Tag :: tag
+begin
+definition "tagName_MyRec_Tag (x::MyRec_Tag) = ''MyRec''"
+instance 
+  by (intro_classes, metis (full_types) Abs_MyRec_Tag_cases singleton_iff)
+end
+
+text {* Next we create a collection of fields associated with the tag, and give each
+        the position in record and its VDM type. *}
+
+abbreviation "maxty_MyRec \<equiv> RecMaximalType \<parallel>@nat*@nat\<parallel> TYPE(MyRec_Tag)"
+
+abbreviation "hgr_fld \<equiv> MkField maxty_MyRec #[1] \<parallel>@nat\<parallel>"
+abbreviation "lwr_fld \<equiv> MkField maxty_MyRec #[2] \<parallel>@nat\<parallel>"
+
+abbreviation "hgr \<equiv> SelectRec hgr_fld"
+abbreviation "lwr  \<equiv> SelectRec lwr_fld"
+
+definition "MyType = \<parallel>[ hgr_fld, lwr_fld] inv x == ^x^.hgr > ^x^.lwr\<parallel>"
+
+term "MyType"
+
+definition "mk_MyType \<equiv> MkRec MyType"
+
+term "|mk_MyType(2,1)|"
+term "|mk_MyType(2,1).lwr|"
+
+lemma "|mk_MyType(2,1) hasType @MyType| = |true|"
+  by (simp add:evalp mk_MyType_def MyType_def vprod_simps)
+
+lemma "|forall x:@nat @ mk_MyType(^x^,0) hasType @MyType| = |false|"
+  by (auto simp add:evalp mk_MyType_def MyType_def vprod_simps)
+*)
+
+end
